LZC.v
@@ -10,22 +10,24 @@ Module Info.
   Definition build_number := "".
   Definition build_tag := "".
   Definition build_branch := "".
-  Definition arch := "x86".
-  Definition model := "64".
-  Definition abi := "standard".
+  Definition arch := "aarch64".
+  Definition model := "default".
+  Definition abi := "apple".
   Definition bitsize := 64.
   Definition big_endian := false.
   Definition source_file := "LZC.c".
   Definition normalized := true.
 End Info.
 
-Definition ___builtin_ais_annot : ident := $"__builtin_ais_annot".
 Definition ___builtin_annot : ident := $"__builtin_annot".
 Definition ___builtin_annot_intval : ident := $"__builtin_annot_intval".
 Definition ___builtin_bswap : ident := $"__builtin_bswap".
 Definition ___builtin_bswap16 : ident := $"__builtin_bswap16".
 Definition ___builtin_bswap32 : ident := $"__builtin_bswap32".
 Definition ___builtin_bswap64 : ident := $"__builtin_bswap64".
+Definition ___builtin_cls : ident := $"__builtin_cls".
+Definition ___builtin_clsl : ident := $"__builtin_clsl".
+Definition ___builtin_clsll : ident := $"__builtin_clsll".
 Definition ___builtin_clz : ident := $"__builtin_clz".
 Definition ___builtin_clzl : ident := $"__builtin_clzl".
 Definition ___builtin_clzll : ident := $"__builtin_clzll".
@@ -45,8 +47,6 @@ Definition ___builtin_fnmsub : ident := $"__builtin_fnmsub".
 Definition ___builtin_fsqrt : ident := $"__builtin_fsqrt".
 Definition ___builtin_membar : ident := $"__builtin_membar".
 Definition ___builtin_memcpy_aligned : ident := $"__builtin_memcpy_aligned".
-Definition ___builtin_read16_reversed : ident := $"__builtin_read16_reversed".
-Definition ___builtin_read32_reversed : ident := $"__builtin_read32_reversed".
 Definition ___builtin_sel : ident := $"__builtin_sel".
 Definition ___builtin_sqrt : ident := $"__builtin_sqrt".
 Definition ___builtin_unreachable : ident := $"__builtin_unreachable".
@@ -54,8 +54,6 @@ Definition ___builtin_va_arg : ident := $"__builtin_va_arg".
 Definition ___builtin_va_copy : ident := $"__builtin_va_copy".
 Definition ___builtin_va_end : ident := $"__builtin_va_end".
 Definition ___builtin_va_start : ident := $"__builtin_va_start".
-Definition ___builtin_write16_reversed : ident := $"__builtin_write16_reversed".
-Definition ___builtin_write32_reversed : ident := $"__builtin_write32_reversed".
 Definition ___compcert_i64_dtos : ident := $"__compcert_i64_dtos".
 Definition ___compcert_i64_dtou : ident := $"__compcert_i64_dtou".
 Definition ___compcert_i64_sar : ident := $"__compcert_i64_sar".
@@ -110,6 +108,7 @@ Definition _out_len : ident := $"out_len".
 Definition _p : ident := $"p".
 Definition _start : ident := $"start".
 Definition _surely_malloc : ident := $"surely_malloc".
+Definition _t : ident := $"t".
 Definition _token_count : ident := $"token_count".
 Definition _t'1 : ident := 128%positive.
 Definition _t'10 : ident := 137%positive.
@@ -153,7 +152,8 @@ Definition f_encode_length := {|
   fn_callconv := cc_default;
   fn_params := ((_len, tulong) :: (_out, (tptr tuchar)) :: nil);
   fn_vars := nil;
-  fn_temps := ((_idx, tulong) :: (_t'2, tulong) :: (_t'1, tulong) :: nil);
+  fn_temps := ((_idx, tulong) :: (_t, tulong) :: (_t'2, tulong) ::
+               (_t'1, tulong) :: nil);
   fn_body :=
 (Ssequence
   (Sifthenelse (Ebinop Oeq (Etempvar _len tulong)
@@ -163,45 +163,50 @@ Definition f_encode_length := {|
   (Ssequence
     (Sset _idx (Ecast (Econst_int (Int.repr 0) tint) tulong))
     (Ssequence
-      (Sloop
+      (Sset _t (Etempvar _len tulong))
+      (Ssequence
+        (Swhile
+          (Ebinop Oge (Etempvar _t tulong) (Econst_int (Int.repr 128) tint)
+            tint)
+          (Ssequence
+            (Ssequence
+              (Ssequence
+                (Sset _t'1 (Etempvar _idx tulong))
+                (Sset _idx
+                  (Ebinop Oadd (Etempvar _t'1 tulong)
+                    (Econst_int (Int.repr 1) tint) tulong)))
+              (Sassign
+                (Ederef
+                  (Ebinop Oadd (Etempvar _out (tptr tuchar))
+                    (Etempvar _t'1 tulong) (tptr tuchar)) tuchar)
+                (Ecast
+                  (Ebinop Oadd
+                    (Ebinop Omod (Etempvar _t tulong)
+                      (Econst_int (Int.repr 128) tint) tulong)
+                    (Econst_int (Int.repr 128) tint) tulong) tuchar)))
+            (Sset _t
+              (Ebinop Odiv (Etempvar _t tulong)
+                (Econst_int (Int.repr 128) tint) tulong))))
         (Ssequence
-          Sskip
-          (Sifthenelse (Ebinop Olt (Etempvar _len tulong)
-                         (Econst_int (Int.repr 128) tint) tint)
+          (Sifthenelse (Ebinop Ogt (Etempvar _t tulong)
+                         (Econst_int (Int.repr 0) tint) tint)
             (Ssequence
               (Ssequence
-                (Ssequence
-                  (Sset _t'1 (Etempvar _idx tulong))
-                  (Sset _idx
-                    (Ebinop Oadd (Etempvar _t'1 tulong)
-                      (Econst_int (Int.repr 1) tint) tulong)))
-                (Sassign
-                  (Ederef
-                    (Ebinop Oadd (Etempvar _out (tptr tuchar))
-                      (Etempvar _t'1 tulong) (tptr tuchar)) tuchar)
-                  (Ecast (Etempvar _len tulong) tuchar)))
-              Sbreak)
-            (Ssequence
-              (Ssequence
-                (Ssequence
-                  (Sset _t'2 (Etempvar _idx tulong))
-                  (Sset _idx
-                    (Ebinop Oadd (Etempvar _t'2 tulong)
-                      (Econst_int (Int.repr 1) tint) tulong)))
-                (Sassign
-                  (Ederef
-                    (Ebinop Oadd (Etempvar _out (tptr tuchar))
-                      (Etempvar _t'2 tulong) (tptr tuchar)) tuchar)
-                  (Ecast
-                    (Ebinop Oadd
-                      (Ebinop Omod (Etempvar _len tulong)
-                        (Econst_int (Int.repr 128) tint) tulong)
-                      (Econst_int (Int.repr 128) tint) tulong) tuchar)))
-              (Sset _len
-                (Ebinop Odiv (Etempvar _len tulong)
-                  (Econst_int (Int.repr 128) tint) tulong)))))
-        Sskip)
-      (Sreturn (Some (Etempvar _idx tulong))))))
+                (Sset _t'2 (Etempvar _idx tulong))
+                (Sset _idx
+                  (Ebinop Oadd (Etempvar _t'2 tulong)
+                    (Econst_int (Int.repr 1) tint) tulong)))
+              (Sassign
+                (Ederef
+                  (Ebinop Oadd (Etempvar _out (tptr tuchar))
+                    (Etempvar _t'2 tulong) (tptr tuchar)) tuchar)
+                (Ecast
+                  (Ebinop Oadd
+                    (Ebinop Omod (Etempvar _t tulong)
+                      (Econst_int (Int.repr 128) tint) tulong)
+                    (Econst_int (Int.repr 128) tint) tulong) tuchar)))
+            Sskip)
+          (Sreturn (Some (Etempvar _idx tulong))))))))
 |}.
 
 Definition f_decode_length := {|
@@ -954,12 +959,6 @@ Definition global_definitions : list (ident * globdef fundef type) :=
                    (mksignature (AST.Xlong :: AST.Xlong :: nil) AST.Xlong
                      cc_default)) (tulong :: tulong :: nil) tulong
      cc_default)) ::
- (___builtin_ais_annot,
-   Gfun(External (EF_builtin "__builtin_ais_annot"
-                   (mksignature (AST.Xptr :: nil) AST.Xvoid
-                     {|cc_vararg:=(Some 1); cc_unproto:=false; cc_structret:=false|}))
-     ((tptr tschar) :: nil) tvoid
-     {|cc_vararg:=(Some 1); cc_unproto:=false; cc_structret:=false|})) ::
  (___builtin_bswap64,
    Gfun(External (EF_builtin "__builtin_bswap64"
                    (mksignature (AST.Xlong :: nil) AST.Xlong cc_default))
@@ -1071,16 +1070,18 @@ Definition global_definitions : list (ident * globdef fundef type) :=
    Gfun(External (EF_builtin "__builtin_expect"
                    (mksignature (AST.Xlong :: AST.Xlong :: nil) AST.Xlong
                      cc_default)) (tlong :: tlong :: nil) tlong cc_default)) ::
- (___builtin_fmax,
-   Gfun(External (EF_builtin "__builtin_fmax"
-                   (mksignature (AST.Xfloat :: AST.Xfloat :: nil) AST.Xfloat
-                     cc_default)) (tdouble :: tdouble :: nil) tdouble
-     cc_default)) ::
- (___builtin_fmin,
-   Gfun(External (EF_builtin "__builtin_fmin"
-                   (mksignature (AST.Xfloat :: AST.Xfloat :: nil) AST.Xfloat
-                     cc_default)) (tdouble :: tdouble :: nil) tdouble
-     cc_default)) ::
+ (___builtin_cls,
+   Gfun(External (EF_builtin "__builtin_cls"
+                   (mksignature (AST.Xint :: nil) AST.Xint cc_default))
+     (tint :: nil) tint cc_default)) ::
+ (___builtin_clsl,
+   Gfun(External (EF_builtin "__builtin_clsl"
+                   (mksignature (AST.Xlong :: nil) AST.Xint cc_default))
+     (tlong :: nil) tint cc_default)) ::
+ (___builtin_clsll,
+   Gfun(External (EF_builtin "__builtin_clsll"
+                   (mksignature (AST.Xlong :: nil) AST.Xint cc_default))
+     (tlong :: nil) tint cc_default)) ::
  (___builtin_fmadd,
    Gfun(External (EF_builtin "__builtin_fmadd"
                    (mksignature
@@ -1105,24 +1106,15 @@ Definition global_definitions : list (ident * globdef fundef type) :=
                      (AST.Xfloat :: AST.Xfloat :: AST.Xfloat :: nil)
                      AST.Xfloat cc_default))
      (tdouble :: tdouble :: tdouble :: nil) tdouble cc_default)) ::
- (___builtin_read16_reversed,
-   Gfun(External (EF_builtin "__builtin_read16_reversed"
-                   (mksignature (AST.Xptr :: nil) AST.Xint16unsigned
-                     cc_default)) ((tptr tushort) :: nil) tushort
+ (___builtin_fmax,
+   Gfun(External (EF_builtin "__builtin_fmax"
+                   (mksignature (AST.Xfloat :: AST.Xfloat :: nil) AST.Xfloat
+                     cc_default)) (tdouble :: tdouble :: nil) tdouble
      cc_default)) ::
- (___builtin_read32_reversed,
-   Gfun(External (EF_builtin "__builtin_read32_reversed"
-                   (mksignature (AST.Xptr :: nil) AST.Xint cc_default))
-     ((tptr tuint) :: nil) tuint cc_default)) ::
- (___builtin_write16_reversed,
-   Gfun(External (EF_builtin "__builtin_write16_reversed"
-                   (mksignature (AST.Xptr :: AST.Xint16unsigned :: nil)
-                     AST.Xvoid cc_default))
-     ((tptr tushort) :: tushort :: nil) tvoid cc_default)) ::
- (___builtin_write32_reversed,
-   Gfun(External (EF_builtin "__builtin_write32_reversed"
-                   (mksignature (AST.Xptr :: AST.Xint :: nil) AST.Xvoid
-                     cc_default)) ((tptr tuint) :: tuint :: nil) tvoid
+ (___builtin_fmin,
+   Gfun(External (EF_builtin "__builtin_fmin"
+                   (mksignature (AST.Xfloat :: AST.Xfloat :: nil) AST.Xfloat
+                     cc_default)) (tdouble :: tdouble :: nil) tdouble
      cc_default)) ::
  (___builtin_debug,
    Gfun(External (EF_external "__builtin_debug"
@@ -1146,26 +1138,24 @@ Definition global_definitions : list (ident * globdef fundef type) :=
 Definition public_idents : list ident :=
 (_main :: _decompress :: _compress :: _find_largest_match ::
  _decode_length :: _encode_length :: _surely_malloc :: _exit :: _malloc ::
- ___builtin_debug :: ___builtin_write32_reversed ::
- ___builtin_write16_reversed :: ___builtin_read32_reversed ::
- ___builtin_read16_reversed :: ___builtin_fnmsub :: ___builtin_fnmadd ::
- ___builtin_fmsub :: ___builtin_fmadd :: ___builtin_fmin ::
- ___builtin_fmax :: ___builtin_expect :: ___builtin_unreachable ::
- ___builtin_va_end :: ___builtin_va_copy :: ___builtin_va_arg ::
- ___builtin_va_start :: ___builtin_membar :: ___builtin_annot_intval ::
- ___builtin_annot :: ___builtin_sel :: ___builtin_memcpy_aligned ::
- ___builtin_sqrt :: ___builtin_fsqrt :: ___builtin_fabsf ::
- ___builtin_fabs :: ___builtin_ctzll :: ___builtin_ctzl :: ___builtin_ctz ::
- ___builtin_clzll :: ___builtin_clzl :: ___builtin_clz ::
- ___builtin_bswap16 :: ___builtin_bswap32 :: ___builtin_bswap ::
- ___builtin_bswap64 :: ___builtin_ais_annot :: ___compcert_i64_umulh ::
- ___compcert_i64_smulh :: ___compcert_i64_sar :: ___compcert_i64_shr ::
- ___compcert_i64_shl :: ___compcert_i64_umod :: ___compcert_i64_smod ::
- ___compcert_i64_udiv :: ___compcert_i64_sdiv :: ___compcert_i64_utof ::
- ___compcert_i64_stof :: ___compcert_i64_utod :: ___compcert_i64_stod ::
- ___compcert_i64_dtou :: ___compcert_i64_dtos :: ___compcert_va_composite ::
- ___compcert_va_float64 :: ___compcert_va_int64 :: ___compcert_va_int32 ::
- nil).
+ ___builtin_debug :: ___builtin_fmin :: ___builtin_fmax ::
+ ___builtin_fnmsub :: ___builtin_fnmadd :: ___builtin_fmsub ::
+ ___builtin_fmadd :: ___builtin_clsll :: ___builtin_clsl :: ___builtin_cls ::
+ ___builtin_expect :: ___builtin_unreachable :: ___builtin_va_end ::
+ ___builtin_va_copy :: ___builtin_va_arg :: ___builtin_va_start ::
+ ___builtin_membar :: ___builtin_annot_intval :: ___builtin_annot ::
+ ___builtin_sel :: ___builtin_memcpy_aligned :: ___builtin_sqrt ::
+ ___builtin_fsqrt :: ___builtin_fabsf :: ___builtin_fabs ::
+ ___builtin_ctzll :: ___builtin_ctzl :: ___builtin_ctz :: ___builtin_clzll ::
+ ___builtin_clzl :: ___builtin_clz :: ___builtin_bswap16 ::
+ ___builtin_bswap32 :: ___builtin_bswap :: ___builtin_bswap64 ::
+ ___compcert_i64_umulh :: ___compcert_i64_smulh :: ___compcert_i64_sar ::
+ ___compcert_i64_shr :: ___compcert_i64_shl :: ___compcert_i64_umod ::
+ ___compcert_i64_smod :: ___compcert_i64_udiv :: ___compcert_i64_sdiv ::
+ ___compcert_i64_utof :: ___compcert_i64_stof :: ___compcert_i64_utod ::
+ ___compcert_i64_stod :: ___compcert_i64_dtou :: ___compcert_i64_dtos ::
+ ___compcert_va_composite :: ___compcert_va_float64 ::
+ ___compcert_va_int64 :: ___compcert_va_int32 :: nil).
 
 Definition prog : Clight.program := 
   mkprogram composites global_definitions public_idents _main Logic.I.
